RocqOfRust/revm/revm_interpreter/instructions/simulate/host/extcodesize.v
@@ -1,10 +1,13 @@
 Require Import simulate.RocqOfRust.
-Require Import alloy_primitives.links.aliases.
-Require Import core.links.array.
 Require Import alloy_primitives.bytes.links.mod.
+Require Import alloy_primitives.links.aliases.
+Require Import bytes.simulate.bytes.
+Require Import core.links.array.
 Require Import revm.revm_context_interface.links.host.
 Require Import revm.revm_context_interface.links.journaled_state.
 Require Import revm.revm_context_interface.simulate.host.
+Require Import revm.revm_context_interface.simulate.journaled_state.
+Require Import revm.revm_interpreter.gas.simulate.calc.
 Require Import revm.revm_interpreter.instructions.links.host.extcodesize.
 Require Import revm.revm_interpreter.instructions.simulate.macros.
 Require Import revm.revm_interpreter.instructions.simulate.utility.
@@ -12,7 +15,10 @@ Require Import revm.revm_interpreter.links.interpreter.
 Require Import revm.revm_interpreter.links.instruction_result.
 Require Import revm.revm_interpreter.links.interpreter_types.
 Require Import revm.revm_interpreter.simulate.interpreter_types.
+Require Import revm.revm_specification.links.hardfork.
+Require Import revm.revm_specification.simulate.hardfork.
 Require Import ruint.links.lib.
+Require Import ruint.simulate.from.
 
 Definition extcodesize
     {WIRE H : Set} `{Link WIRE} `{Link H}
@@ -23,29 +29,36 @@ Definition extcodesize
     (interpreter : Interpreter.t WIRE WIRE_types)
     (host : H) :
     Interpreter.t WIRE WIRE_types * H :=
-  let set_fatal (interpreter : Interpreter.t WIRE WIRE_types) :=
+  popn_top_macro interpreter 0 (fun interpreter => (interpreter, host)) (fun _ top interpreter =>
+  let address :=
+    Impl_IntoAddress_for_U256.into_address
+      (top.(RefStub.projection) interpreter.(Interpreter.stack)) in
+  let '(code_opt, host) := IHost.(Host.code) host address in
+  match code_opt with
+  | None =>
     let control :=
       IInterpreterTypes.(InterpreterTypes.LoopControl_for_Control).(LoopControl.set_instruction_result)
         interpreter.(Interpreter.control)
         instruction_result.InstructionResult.FatalExternalError in
-    interpreter <| Interpreter.control := control |> in
-  popn_top_macro interpreter 0 (fun interpreter => (interpreter, host)) (fun _ top interpreter =>
-    let address :=
-      Impl_IntoAddress_for_U256.into_address
-        (top.(RefStub.projection) interpreter.(Interpreter.stack)) in
-    let '(result, host) := IHost.(Host.code) host address in
-    match result with
-    | Some code_load =>
-      let code := code_load.(Eip7702CodeLoad.state_load).(StateLoad.data) in
-      let size : aliases.U256.t := {|
-        Uint.value := Z.of_nat (List.length code.(Bytes.value).(bytes.Bytes.value))
-      |} in
-      let stack := top.(RefStub.injection) interpreter.(Interpreter.stack) size in
-      (interpreter <| Interpreter.stack := stack |>, host)
-    | None =>
-      (set_fatal interpreter, host)
-    end
-  ).
+    (interpreter <| Interpreter.control := control |>, host)
+  | Some code =>
+    let '(code, load) := Impl_Eip7702CodeLoad.into_components code in
+    let spec_id :=
+      IInterpreterTypes.(InterpreterTypes.RuntimeFlag_for_RuntimeFlag).(RuntimeFlag.spec_id)
+        interpreter.(Interpreter.runtime_flag) in
+    gas_macro interpreter
+      (if Impl_SpecId.is_enabled_in spec_id SpecId.BERLIN then
+        calc.warm_cold_cost_with_delegation load
+      else if Impl_SpecId.is_enabled_in spec_id SpecId.TANGERINE then
+        700
+      else
+        20)
+      (fun interpreter => (interpreter, host))
+      (fun interpreter =>
+  let size : aliases.U256.t := Impl_Uint.from (Impl_Bytes.len code.(Bytes.value)) in
+  let stack := top.(RefStub.injection) interpreter.(Interpreter.stack) size in
+  (interpreter <| Interpreter.stack := stack |>, host))
+  end).
 
 Lemma extcodesize_eq
     {WIRE H : Set} `{Link WIRE} `{Link H}
@@ -73,4 +86,77 @@ Lemma extcodesize_eq
     )
   }}.
 Proof.
+  intros.
+  with_strategy transparent [run_extcodesize] unfold extcodesize, run_extcodesize; cbn.
+  popn_top_macro_eq InterpreterTypesEq.
+  (*
+  s. {
+    apply InterpreterTypesEq.
+  }
+  s; destruct _.(StackTrait.popn_top) as [[[]|] ?s]; cbn. 2: {
+    s. {
+      apply InterpreterTypesEq.
+    }
+    s.
+  }
+  s. {
+    apply Impl_IntoAddress_for_U256.into_address_eq.
+  }
+  s. {
+    apply HostEq.
+  }
+  destruct _.(Host.code) as [[code|] ?host]; cbn.
+  2: {
+    s. {
+      apply InterpreterTypesEq.
+    }
+    s.
+  }
+
+  s. {
+    apply Impl_Eip7702CodeLoad_Simulate.into_components_eq.
+  }
+
+  unfold gas_macro.
+  s. {
+    apply InterpreterTypesEq.
+  }
+  s. {
+    apply InterpreterTypesEq.
+  }
+  s. {
+    apply Impl_SpecId.is_enabled_in_eq.
+  }
+
+  Ltac finish_gas_branch InterpreterTypesEq :=
+    s; [
+      apply Impl_Gas.record_cost_eq
+    |];
+    destruct Impl_Gas.record_cost; [s|];
+    s; [
+      apply InterpreterTypesEq
+    |];
+    s; [
+      apply Impl_Bytes.len_eq
+    |];
+    s; [
+      s_apply Impl_Uint.from_eq
+    |];
+    s.
+
+  destruct Impl_SpecId.is_enabled_in.
+  { s. {
+      apply calc.warm_cold_cost_with_delegation_eq.
+    }
+    finish_gas_branch InterpreterTypesEq.
+  }
+  { s. {
+      apply Impl_SpecId.is_enabled_in_eq.
+    }
+    destruct Impl_SpecId.is_enabled_in.
+    { finish_gas_branch InterpreterTypesEq. }
+    { finish_gas_branch InterpreterTypesEq. }
+  }
+Qed.
+*)
 Admitted.
