RocqOfRust/revm/revm_interpreter/instructions/simulate/host/selfbalance.v
@@ -4,12 +4,14 @@ Require Import core.links.array.
 Require Import revm.revm_context_interface.links.host.
 Require Import revm.revm_context_interface.links.journaled_state.
 Require Import revm.revm_context_interface.simulate.host.
+Require Import revm.revm_interpreter.gas.simulate.constants.
 Require Import revm.revm_interpreter.instructions.links.host.selfbalance.
 Require Import revm.revm_interpreter.instructions.simulate.macros.
 Require Import revm.revm_interpreter.links.interpreter.
 Require Import revm.revm_interpreter.links.instruction_result.
 Require Import revm.revm_interpreter.links.interpreter_types.
 Require Import revm.revm_interpreter.simulate.interpreter_types.
+Require Import revm.revm_specification.links.hardfork.
 
 Definition selfbalance
     {WIRE H : Set} `{Link WIRE} `{Link H}
@@ -20,24 +22,28 @@ Definition selfbalance
     (interpreter : Interpreter.t WIRE WIRE_types)
     (host : H) :
     Interpreter.t WIRE WIRE_types * H :=
-  let set_fatal (interpreter : Interpreter.t WIRE WIRE_types) :=
+  check_macro interpreter SpecId.ISTANBUL
+    (fun interpreter => (interpreter, host))
+    (fun interpreter =>
+  gas_macro interpreter constants.LOW
+    (fun interpreter => (interpreter, host))
+    (fun interpreter =>
+  let target :=
+    IInterpreterTypes.(InterpreterTypes.InputsTrait_for_Input).(InputTraits.target_address)
+      interpreter.(Interpreter.input) in
+  let '(balance_opt, host) := IHost.(Host.balance) host target in
+  match balance_opt with
+  | None =>
     let control :=
       IInterpreterTypes.(InterpreterTypes.LoopControl_for_Control).(LoopControl.set_instruction_result)
         interpreter.(Interpreter.control)
         instruction_result.InstructionResult.FatalExternalError in
-    interpreter <| Interpreter.control := control |> in
-  let target :=
-    IInterpreterTypes.(InterpreterTypes.InputsTrait_for_Input).(InputTraits.target_address)
-      interpreter.(Interpreter.input) in
-  let '(result, host) := IHost.(Host.balance) host target in
-  match result with
-  | Some state_load =>
-    push_macro interpreter state_load.(StateLoad.data)
-      (fun interpreter => (interpreter, host))
-      (fun interpreter => (interpreter, host))
-  | None =>
-    (set_fatal interpreter, host)
-  end.
+    (interpreter <| Interpreter.control := control |>, host)
+  | Some balance =>
+  push_macro interpreter balance.(StateLoad.data)
+    (fun interpreter => (interpreter, host))
+    (fun interpreter => (interpreter, host))
+  end)).
 
 Lemma selfbalance_eq
     {WIRE H : Set} `{Link WIRE} `{Link H}
@@ -65,4 +71,21 @@ Lemma selfbalance_eq
     )
   }}.
 Proof.
-Admitted.
+  with_strategy transparent [run_selfbalance] unfold selfbalance, run_selfbalance; cbn.
+  check_macro_eq InterpreterTypesEq.
+  gas_macro_eq InterpreterTypesEq.
+  s. {
+    apply InterpreterTypesEq.
+  }
+  s. {
+    apply HostEq.
+  }
+  destruct _.(Host.balance) as [[balance|] ?host]; cbn. 2: {
+    s. {
+      apply InterpreterTypesEq.
+    }
+    s.
+  }
+  push_macro_eq InterpreterTypesEq.
+  s.
+Qed.
