RocqOfRust/revm/revm_context_interface/simulate/journaled_state.v
@@ -1,0 +1,82 @@
+Require Import simulate.RocqOfRust.
+Require Import core.ops.links.deref.
+Require Import core.ops.simulate.deref.
+Require Import revm.revm_context_interface.links.journaled_state.
+
+Module Impl_Deref_for_StateLoad.
+  Definition Self (T : Set) : Set :=
+    StateLoad.t T.
+
+  Definition deref {T : Set} `{Link T} : RefStub.t (Self T) T := {|
+    RefStub.path := [];
+    RefStub.projection x := x.(StateLoad.data);
+    RefStub.injection x y := x <| StateLoad.data := y |>;
+  |}.
+
+  Lemma deref_eq
+      {T : Set} `{Link T}
+      (ref_self : '& (Self T))
+      (self : Self T)
+      (stack : Stack.t) :
+    CanRead.t stack self ref_self ->
+    {{
+      SimulateM.eval_f
+        (Deref.run_deref ref_self)
+        stack 🌲
+      (
+        Output.Success (RefStub.apply ref_self deref),
+        stack
+      )
+    }}.
+  Admitted.
+
+  Instance I {T : Set} `{Link T} :
+      core.ops.simulate.deref.Deref.C (Self T) T := {|
+    core.ops.simulate.deref.Deref.deref := deref;
+  |}.
+
+  Module Eq.
+    Instance I {T : Set} `{Link T} :
+      core.ops.simulate.deref.Deref.Eq.t
+        (Self := Self T) (Target := T) Impl_Deref_for_StateLoad.I.
+    Proof.
+    Admitted.
+  End Eq.
+  Export (hints) Eq.
+End Impl_Deref_for_StateLoad.
+Export (hints) Impl_Deref_for_StateLoad.
+
+Module Impl_Eip7702CodeLoad.
+  Definition Self (T : Set) : Set :=
+    Eip7702CodeLoad.t T.
+
+  Definition into_components {T : Set} (self : Self T) : T * Self unit :=
+    (
+      self.(Eip7702CodeLoad.state_load).(StateLoad.data),
+      {|
+        Eip7702CodeLoad.state_load := {|
+          StateLoad.data := tt;
+          StateLoad.is_cold :=
+            self.(Eip7702CodeLoad.state_load).(StateLoad.is_cold);
+        |};
+        Eip7702CodeLoad.is_delegate_account_cold :=
+          self.(Eip7702CodeLoad.is_delegate_account_cold);
+      |}
+    ).
+
+  Lemma into_components_eq
+      {T : Set} `{Link T}
+      (self : Self T)
+      (stack : Stack.t) :
+    {{
+      SimulateM.eval_f
+        (@Impl_Eip7702CodeLoad.run_into_components T _ self)
+        stack 🌲
+      (
+        Output.Success (into_components self),
+        stack
+      )
+    }}.
+  Admitted.
+End Impl_Eip7702CodeLoad.
+Export (hints) Impl_Eip7702CodeLoad.
