RocqOfRust/revm/revm_interpreter/instructions/simulate/block_info/chainid.v
@@ -1,0 +1,79 @@
+Require Import simulate.RocqOfRust.
+Require Import alloy_primitives.links.aliases.
+Require Import revm.revm_context_interface.links.host.
+Require Import revm.revm_context_interface.simulate.cfg.
+Require Import revm.revm_context_interface.simulate.host.
+Require Import revm.revm_interpreter.gas.simulate.constants.
+Require Import revm.revm_interpreter.instructions.links.block_info.
+Require Import revm.revm_interpreter.instructions.simulate.macros.
+Require Import revm.revm_interpreter.links.gas.
+Require Import revm.revm_interpreter.links.interpreter.
+Require Import revm.revm_interpreter.links.interpreter_types.
+Require Import revm.revm_interpreter.simulate.gas.
+Require Import revm.revm_interpreter.simulate.interpreter_types.
+Require Import revm.revm_specification.links.hardfork.
+Require Import revm.revm_specification.simulate.hardfork.
+Require Import ruint.links.lib.
+Require Import ruint.simulate.from.
+
+Definition chainid
+    {WIRE H : Set} `{Link WIRE} `{Link H}
+    {WIRE_types : InterpreterTypes.Types.t} `{InterpreterTypes.Types.AreLinks WIRE_types}
+    {IInterpreterTypes : InterpreterTypes.C WIRE_types}
+    {H_types : Host.Types.t} `{Host.Types.AreLinks H_types}
+    {IHost : Host.C H H_types}
+    (interpreter : Interpreter.t WIRE WIRE_types)
+    (host : H) :
+    Interpreter.t WIRE WIRE_types * H :=
+  check_macro interpreter SpecId.ISTANBUL (fun interpreter => (interpreter, host)) (fun interpreter =>
+  gas_macro interpreter constants.BASE (fun interpreter => (interpreter, host)) (fun interpreter =>
+  let cfg := IHost.(Host.CfgGetter_for_Self).(CfgGetter.cfg).(RefStub.projection) host in
+  let chain_id := IHost.(Host.CfgGetter_for_Self).(CfgGetter.Cfg_for_Cfg).(Cfg.chain_id) cfg in
+  push_macro interpreter
+    {| Uint.value := i[chain_id] |}
+    (fun interpreter => (interpreter, host)) (fun interpreter =>
+  (interpreter, host)
+  ))).
+
+Lemma chainid_eq
+    {WIRE H : Set} `{Link WIRE} `{Link H}
+    {WIRE_types : InterpreterTypes.Types.t} `{InterpreterTypes.Types.AreLinks WIRE_types}
+    {H_types : Host.Types.t} `{Host.Types.AreLinks H_types}
+    (run_InterpreterTypes_for_WIRE : InterpreterTypes.Run WIRE WIRE_types)
+    (run_Host_for_H : Host.Run H H_types)
+    (IInterpreterTypes : InterpreterTypes.C WIRE_types)
+    (InterpreterTypesEq :
+      InterpreterTypes.Eq.t WIRE WIRE_types run_InterpreterTypes_for_WIRE IInterpreterTypes)
+    (IHost : Host.C H H_types)
+    (HostEq : Host.Eq.t IHost)
+    (interpreter : Interpreter.t WIRE WIRE_types)
+    (host : H) :
+  let ref_interpreter : '&mut (Interpreter.t WIRE WIRE_types) := make_ref 0 in
+  let ref_host : '&mut H := make_ref 1 in
+  {{
+    SimulateM.eval_f
+      (run_chainid run_InterpreterTypes_for_WIRE run_Host_for_H ref_interpreter ref_host)
+      ([interpreter; host]%stack) 🌲
+    (
+      Output.Success tt,
+      let '(interpreter, host) := chainid interpreter host in
+      [interpreter; host]%stack
+    )
+  }}.
+Proof.
+  intros.
+  with_strategy transparent [run_chainid] unfold chainid, run_chainid; cbn.
+  check_macro_eq InterpreterTypesEq.
+  gas_macro_eq InterpreterTypesEq.
+  s. {
+    apply HostEq.
+  }
+  s. {
+    s_apply HostEq.
+  }
+  s. {
+    s_apply Impl_Uint.from_eq.
+  }
+  push_macro_eq InterpreterTypesEq.
+  s.
+Qed.
