RocqOfRust/revm/revm_interpreter/instructions/simulate/block_info/difficulty.v
@@ -1,0 +1,119 @@
+Require Import simulate.RocqOfRust.
+Require Import alloy_primitives.bits.links.fixed.
+Require Import alloy_primitives.links.aliases.
+Require Import core.simulate.option.
+Require Import revm.revm_context_interface.links.host.
+Require Import revm.revm_context_interface.simulate.block.
+Require Import revm.revm_context_interface.simulate.host.
+Require Import revm.revm_interpreter.gas.simulate.constants.
+Require Import revm.revm_interpreter.instructions.links.block_info.
+Require Import revm.revm_interpreter.instructions.simulate.macros.
+Require Import revm.revm_interpreter.instructions.simulate.utility.
+Require Import revm.revm_interpreter.links.gas.
+Require Import revm.revm_interpreter.links.interpreter.
+Require Import revm.revm_interpreter.links.interpreter_types.
+Require Import revm.revm_interpreter.simulate.gas.
+Require Import revm.revm_interpreter.simulate.interpreter_types.
+Require Import revm.revm_specification.links.hardfork.
+Require Import revm.revm_specification.simulate.hardfork.
+Require Import ruint.links.lib.
+Require Import ruint.simulate.lib.
+
+Definition difficulty
+    {WIRE H : Set} `{Link WIRE} `{Link H}
+    {WIRE_types : InterpreterTypes.Types.t} `{InterpreterTypes.Types.AreLinks WIRE_types}
+    {IInterpreterTypes : InterpreterTypes.C WIRE_types}
+    {H_types : Host.Types.t} `{Host.Types.AreLinks H_types}
+    {IHost : Host.C H H_types}
+    (interpreter : Interpreter.t WIRE WIRE_types)
+    (host : H) :
+    Interpreter.t WIRE WIRE_types * H :=
+  gas_macro interpreter constants.BASE (fun interpreter => (interpreter, host)) (fun interpreter =>
+  let spec_id :=
+    IInterpreterTypes.(InterpreterTypes.RuntimeFlag_for_RuntimeFlag).(RuntimeFlag.spec_id)
+      interpreter.(Interpreter.runtime_flag) in
+  let block :=
+    IHost.(Host.BlockGetter_for_Self).(BlockGetter.block).(RefStub.projection) host in
+  let is_merge := Impl_SpecId.is_enabled_in spec_id SpecId.MERGE in
+  let value :=
+    if is_merge then
+      match IHost.(Host.BlockGetter_for_Self).(BlockGetter.Block_for_Block).(Block.prevrandao) block with
+      | Some prevrandao => Impl_IntoU256_for_B256.into_u256 prevrandao
+      | None => Impl_Uint.ZERO
+      end
+    else
+      IHost.(Host.BlockGetter_for_Self).(BlockGetter.Block_for_Block).(Block.difficulty) block
+  in
+  push_macro interpreter value (fun interpreter => (interpreter, host)) (fun interpreter =>
+  (interpreter, host)
+  )).
+
+Lemma difficulty_eq
+    {WIRE H : Set} `{Link WIRE} `{Link H}
+    {WIRE_types : InterpreterTypes.Types.t} `{InterpreterTypes.Types.AreLinks WIRE_types}
+    {H_types : Host.Types.t} `{Host.Types.AreLinks H_types}
+    (run_Host_for_H : Host.Run H H_types)
+    (run_InterpreterTypes_for_WIRE : InterpreterTypes.Run WIRE WIRE_types)
+    (IInterpreterTypes : InterpreterTypes.C WIRE_types)
+    (InterpreterTypesEq :
+      InterpreterTypes.Eq.t WIRE WIRE_types run_InterpreterTypes_for_WIRE IInterpreterTypes)
+    (IHost : Host.C H H_types)
+    (HostEq : Host.Eq.t IHost)
+    (interpreter : Interpreter.t WIRE WIRE_types)
+    (host : H)
+    (prevrandao : FixedBytes.t 32)
+    (H_prevrandao :
+      IHost.(Host.BlockGetter_for_Self).(BlockGetter.Block_for_Block).(Block.prevrandao)
+        (IHost.(Host.BlockGetter_for_Self).(BlockGetter.block).(RefStub.projection) host) =
+      Some prevrandao
+    ) :
+  let ref_interpreter : '&mut (Interpreter.t WIRE WIRE_types) := make_ref 0 in
+  let ref_host : '&mut H := make_ref 1 in
+  {{
+    SimulateM.eval_f
+      (run_difficulty run_Host_for_H run_InterpreterTypes_for_WIRE ref_interpreter ref_host)
+      ([interpreter; host]%stack) 🌲
+    (
+      Output.Success tt,
+      let '(interpreter, host) := difficulty interpreter host in
+      [interpreter; host]%stack
+    )
+  }}.
+Proof.
+  intros.
+  with_strategy transparent [run_difficulty] unfold difficulty, run_difficulty; cbn.
+  gas_macro_eq InterpreterTypesEq.
+  s. {
+    apply InterpreterTypesEq.
+  }
+  s. {
+    apply Impl_SpecId.is_enabled_in_eq.
+  }
+  destruct Impl_SpecId.is_enabled_in; cbn.
+  { s. {
+      apply HostEq.
+    }
+    s. {
+      s_apply HostEq.
+    }
+    s. {
+      apply Impl_Option.unwrap_eq.
+      exact H_prevrandao.
+    }
+    s. {
+      apply Impl_IntoU256_for_B256.into_u256_eq.
+    }
+    rewrite H_prevrandao.
+    push_macro_eq InterpreterTypesEq.
+    s.
+  }
+  { s. {
+      apply HostEq.
+    }
+    s. {
+      s_apply HostEq.
+    }
+    push_macro_eq InterpreterTypesEq.
+    s.
+  }
+Qed.
